coq/NetCore/NetCoreCompiler.v
@@ -32,7 +32,7 @@ Fixpoint desugar_pred (p : predicate) := match p with
 end.
 
 Fixpoint compile_pred (opt : Classifier bool -> Classifier bool) 
-         (pr : Pred) (sw : switchId) : Classifier bool := 
+         (pr : pred) (sw : switchId) : Classifier bool := 
   match pr with
     | PrHdr pat => [(pat, true)]
     | PrOnSwitch sw' => 
@@ -74,19 +74,19 @@ Fixpoint desugar_pol' p pr :=
 
 Definition desugar_pol (p : policy) := desugar_pol' p All.
 
-Definition apply_act (a : list Action) (b : bool) := 
+Definition apply_act (a : list act) (b : bool) := 
   match b with
     | true => a
     | false => nil
   end.
 
 (** TODO(arjun): rank-2 polymorphism. The extracted code makes me nervous. *)
-Fixpoint compile_pol (opt : forall (A : Type), Classifier A -> Classifier A) (p : Pol) (sw : switchId) : Classifier (list Action) :=
+Fixpoint compile_pol (opt : forall (A : Type), Classifier A -> Classifier A) (p : pol) (sw : switchId) : Classifier (list act) :=
   match p with
     | PoAtom pr act => 
       opt _ (map (second (apply_act act)) (compile_pred (opt bool) pr sw ++ [(Pattern.all, false)]))
     | PoUnion pol1 pol2 => 
-      opt _ (union (@app Action) (compile_pol opt pol1 sw) (compile_pol opt pol2 sw))
+      opt _ (union (@app act) (compile_pol opt pol1 sw) (compile_pol opt pol2 sw))
   end.
 
 Fixpoint strip_empty_rules (A : Type) (cf : Classifier A) : Classifier A :=
@@ -98,7 +98,7 @@ Fixpoint strip_empty_rules (A : Type) (cf : Classifier A) : Classifier A :=
       else (pat, acts) :: strip_empty_rules cf
   end.
 
-Definition no_opt (A : Type) := @id (Classifier A).
+Definition no_opt (A : Type) := @Datatypes.id (Classifier A).
 
 Definition compile_no_opt := compile_pol no_opt.
 
